Optimizations/Canonicalizations/BinaryNode.thy
@@ -8,7 +8,6 @@ phase BinaryNde
 begin
 
 optimization BinaryFoldConstant: "BinaryExpr op (const v1) (const v2) \<longmapsto> ConstantExpr (bin_eval op v1 v2)"
-  apply (cases op; simp)
   unfolding le_expr_def
   apply (rule allI impI)+
   subgoal premises bin for m p v
