Optimizations/Canonicalizations/OrPhase.thy
@@ -1,7 +1,6 @@
 theory OrPhase
   imports
     Common
-    NewAnd (* Allows access to mask operations *)
 begin
 
 section \<open>Optimizations for Or Nodes\<close>
@@ -33,7 +32,7 @@ lemma val_or_equal:
 
 lemma val_elim_redundant_false:
   assumes "x = new_int b v"
-  assumes "x \<noteq> UndefVal \<and> (intval_or x (bool_to_val False)) \<noteq> UndefVal"
+  assumes "val[x | false] \<noteq> UndefVal"
   shows "val[x | false] = val[x]"
    using assms apply (cases x; auto) by presburger
 
@@ -50,41 +49,49 @@ lemma val_or_not_operands:
 (* Expr level proofs *)
 lemma exp_or_equal:
   "exp[x | x] \<ge> exp[x]"
-   apply simp using val_or_equal sorry (*
-  by (metis bin_eval.simps(5) evalDet evaltree_not_undef unfold_binary)*)
+   using val_or_equal apply auto
+   by (smt (verit, ccfv_SIG) evalDet eval_unused_bits_zero intval_negate.elims intval_or.simps(2) intval_or.simps(6) intval_or.simps(7) new_int.simps val_or_equal)
 
 lemma exp_elim_redundant_false:
  "exp[x | false] \<ge> exp[x]"
-   apply simp using val_elim_redundant_false 
-   apply (cases x) sorry (*
-  by (metis BinaryExprE bin_eval.simps(5) bool_to_val.simps(2) evaltree_not_undef)+*)
-  
+   using val_elim_redundant_false apply auto
+   by (smt (verit) Value.sel(1) eval_unused_bits_zero intval_or.elims new_int.simps new_int_bin.simps val_elim_redundant_false)
+
+
 (* Optimizations *)
 optimization OrEqual: "x | x \<longmapsto> x"
   by (meson exp_or_equal le_expr_def)
 
 
 optimization OrShiftConstantRight: "((const x) | y) \<longmapsto> y | (const x) when \<not>(is_ConstantExpr y)"
-   unfolding le_expr_def using val_shift_const_right_helper size_non_const
-   apply simp apply auto 
-  sorry
+  using size_non_const apply force
+  apply auto
+  by (simp add: BinaryExpr unfold_const val_shift_const_right_helper)
 
 optimization EliminateRedundantFalse: "x | false \<longmapsto> x"
   by (meson exp_elim_redundant_false le_expr_def)
 
 
-optimization OrNotOperands: "(~x | ~y) \<longmapsto> ~ (x & y)"
+optimization OrNotOperands: "(~x | ~y) \<longmapsto> ~(x & y)"
+  defer
    apply auto using val_or_not_operands
-  by (metis BinaryExpr UnaryExpr bin_eval.simps(4) intval_not.simps(2) unary_eval.simps(3))
-
-optimization OrLeftFallthrough: "(x | y) \<longmapsto> x
-                                when (((and (not (IRExpr_down x)) (IRExpr_up y)) = 0))"
-  by (simp add: IRExpr_down_def IRExpr_up_def) 
-
-optimization OrRightFallthrough: "(x | y) \<longmapsto> y
-                                when (((and (not (IRExpr_down y)) (IRExpr_up x)) = 0))"
-  by (meson exp_or_commute OrLeftFallthrough(1) order.trans rewrite_preservation.simps(2))
+  apply (metis BinaryExpr UnaryExpr bin_eval.simps(4) intval_not.simps(2) unary_eval.simps(3))
+  sorry (* termination *)
 
 end (* End of OrPhase *)
+
+
+context stamp_mask
+begin
+
+lemma OrLeftFallthrough:
+  assumes "(and (not (\<down>x)) (\<up>y)) = 0"
+  shows "exp[x | y] \<ge> exp[x]"
+  using assms sorry
+
+lemma OrRightFallthrough: 
+  assumes "(and (not (\<down>y)) (\<up>x)) = 0"
+  shows "exp[x | y] \<ge> exp[y]"
+  using assms sorry
 
 end (* End of file *)
