Optimizations/Canonicalizations/SignedRemPhase.thy
@@ -11,8 +11,8 @@ begin
 
 
 lemma val_remainder_one:
-  assumes "intval_mod x (IntVal32 1) \<noteq> UndefVal"
-  shows "intval_mod x (IntVal32 1) = IntVal32 0"
+  assumes "intval_mod x (IntVal 32 1) \<noteq> UndefVal"
+  shows "intval_mod x (IntVal 32 1) = IntVal 32 0"
   using assms apply (cases x; auto) sorry
   
 value "word_of_int (sint (x2::32 word) smod 1)"
